common/Memtype.v
@@ -186,14 +186,14 @@ that we now axiomatize. *)
  stack_adt: mem -> stack_adt;
  (* Pushes a new stage on the stack, with no frames in it. *)
  push_new_stage: mem -> mem;
- record_stack_blocks: mem -> frame_adt -> mem -> Prop;
+ record_stack_blocks: mem -> frame_adt -> option mem;
  (* record_stack_blocks_tailcall: mem -> frame_adt -> mem -> Prop; *)
- push_frame: mem -> frame_info -> list (memory_chunk * ptrofs * val) -> option (mem*block);
- record_stack_blocks_none: forall (m: mem) (bl : list (block * frame_info)) (sz: Z),
-                           Forall
-                             (fun b : block * frame_info =>
-                                forall (o : Z) (k : perm_kind) (p : permission), perm m (fst b) o k p -> 0 <= o < frame_size (snd b)) bl -> 
-                           option mem;
+ (* push_frame: mem -> frame_info -> list (memory_chunk * ptrofs * val) -> option (mem*block); *)
+ (* record_stack_blocks_none: forall (m: mem) (bl : list (block * frame_info)) (sz: Z), *)
+ (*                           Forall *)
+ (*                             (fun b : block * frame_info => *)
+ (*                                forall (o : Z) (k : perm_kind) (p : permission), perm m (fst b) o k p -> 0 <= o < frame_size (snd b)) bl ->  *)
+ (*                           option mem; *)
  unrecord_stack_block: mem -> option mem;
  frame_inject f := StackADT.frame_inject f;
  stack_limit: Z;
@@ -217,16 +217,6 @@ Definition storev (chunk: memory_chunk) (m: mem) (addr v: val) : option mem :=
   match addr with
   | Vptr b ofs => store chunk m b (Ptrofs.unsigned ofs) v
   | _ => None
-  end.
-
-Fixpoint do_stores (m: mem) (l: list (memory_chunk * val * val)) : option mem :=
-  match l with
-    nil => Some m
-  | (k,addr,v)::r =>
-    match storev k m addr v with
-      Some m1 => do_stores m1 r
-    | None => None
-    end
   end.
 
 (** [free_list] frees all the given (block, lo, hi) triples. *)
@@ -1677,7 +1667,7 @@ for [unchanged_on]. *)
      (FAP1: frame_at_pos (stack_adt m1) 0 tf1)
      (FAP2: frame_at_pos (stack_adt m2) 0 f2)
      (FI: tframe_inject j (f1::tf1) f2)
-     (RSB: record_stack_blocks m1 f1 m1'),
+     (RSB: record_stack_blocks m1 f1 = Some m1'),
      inject j (fun n : nat => if Nat.eq_dec n 0 then Some O else g (Init.Nat.pred n)) m1' m2;
 
  record_stack_blocks_inject_parallel {injperm: InjectPerm}:
@@ -1690,17 +1680,17 @@ for [unchanged_on]. *)
               forall o k p, perm m2 b o k p -> 0 <= o < frame_size fi) ->
      (forall (b1 b2 : block) (delta : Z), j b1 = Some (b2, delta) -> in_frame fi1 b1 <-> in_frame fi2 b2) ->
      frame_adt_size fi1 = frame_adt_size fi2 ->
-     record_stack_blocks m1 fi1 m1' ->
+     record_stack_blocks m1 fi1 = Some m1' ->
      top_tframe_no_perm (perm m2) (stack_adt m2) ->
      exists m2',
-       record_stack_blocks m2 fi2 m2' /\
+       record_stack_blocks m2 fi2 = Some m2' /\
        inject j (fun n => if Nat.eq_dec n 0 then Some O else option_map S (g (pred n))) m1' m2';
 
 
  record_stack_blocks_extends {injperm: InjectPerm}:
     forall m1 m2 m1' fi,
       extends m1 m2 ->
-      record_stack_blocks m1 fi m1' ->
+      record_stack_blocks m1 fi = Some m1' ->
       (forall b, in_frame fi b -> ~ in_stack ( (stack_adt m2)) b ) ->
       Forall
         (fun b : block * frame_info =>
@@ -1709,23 +1699,23 @@ for [unchanged_on]. *)
         (frame_adt_blocks fi) ->
       top_tframe_no_perm (perm m2) (stack_adt m2) ->
       exists m2',
-        record_stack_blocks m2 fi m2' /\
+        record_stack_blocks m2 fi = Some m2' /\
         extends m1' m2';
 
  record_stack_blocks_mem_unchanged:
    forall bfi,
-     mem_unchanged (fun m1 m2 => record_stack_blocks m1 bfi m2);
+     mem_unchanged (fun m1 m2 => record_stack_blocks m1 bfi = Some m2);
 
  record_stack_blocks_stack_adt:
    forall m fi m' f s,
-     record_stack_blocks m fi m' ->
+     record_stack_blocks m fi = Some m' ->
      stack_adt m = f::s ->
      stack_adt m' = (fi :: f) :: s;
 
  record_stack_blocks_inject_neutral {injperm: InjectPerm}:
    forall thr m fi m',
      inject_neutral thr m ->
-     record_stack_blocks m fi m' ->
+     record_stack_blocks m fi = Some m' ->
      Forall (fun b => Plt b thr) (map fst (frame_adt_blocks fi)) ->
      inject_neutral thr m';
 
@@ -1858,31 +1848,6 @@ for [unchanged_on]. *)
    forall m, size_stack (stack_adt m) < stack_limit;
 
  
- push_frame_alloc_record:
-   forall m1 b fi l m4 fa,
-     push_frame m1 fi l = Some (m4,b) ->
-     frame_adt_blocks fa = (b,fi)::nil ->
-     frame_adt_size fa = Z.max 0 (frame_size fi) ->
-     exists m2,
-       alloc m1 0 (frame_size fi) = (m2, b) /\
-       exists m3,
-         do_stores m2 (store_spec_of_ofs_spec b l) = Some m3 /\
-         record_stack_blocks (push_new_stage m3) fa m4;
-
- alloc_record_push_frame:
-   forall m1 m2 b fi l m3 m4 fa,
-     frame_adt_blocks fa = (b,fi)::nil ->
-     frame_adt_size fa = Z.max 0 (frame_size fi) ->
-     alloc m1 0 (frame_size fi) = (m2, b) ->
-     do_stores m2 (store_spec_of_ofs_spec b l) = Some m3 ->
-     record_stack_blocks (push_new_stage m3) fa m4 ->
-     push_frame m1 fi l = Some (m4,b);
-
- record_stack_blocks_none_correct:
-   forall m (bl: list (block * frame_info)) sz m',
-     (exists pf, record_stack_blocks_none m bl sz pf = Some m') <->
-     (exists fa, record_stack_blocks m fa m' /\ frame_adt_blocks fa = bl /\ frame_adt_size fa = Z.max 0 sz);
-
  record_stack_block_inject_left_zero {injperm: InjectPerm}:
     forall m1 m1' m2 j g tf1 f1 f2
       (INJ: inject j g m1 m2)
@@ -1890,7 +1855,7 @@ for [unchanged_on]. *)
       (FAP2: frame_at_pos (stack_adt m2) O f2)
       (FI: tframe_inject j (f1::tf1) f2)
       (SZ2: Forall (fun f => Forall (fun f =>0 = frame_adt_size f) f)%Z (stack_adt m2)) 
-      (RSB: record_stack_blocks m1 f1 m1'),
+      (RSB: record_stack_blocks m1 f1 = Some m1'),
       inject j (fun n : nat => if Nat.eq_dec n O then Some O else g (pred n)) m1' m2;
 
  unrecord_stack_block_inject_left_zero {injperm: InjectPerm}:
@@ -1921,13 +1886,7 @@ for [unchanged_on]. *)
       (size_stack (stack_adt m1) + align (frame_adt_size f) 8 < stack_limit)%Z ->
       top_tframe_no_perm (perm m1) (stack_adt m1) ->
       exists m2,
-        record_stack_blocks m1 f m2;
-
- record_stack_block_det:
-   forall m f m1 m2,
-     record_stack_blocks m f m1 ->
-     record_stack_blocks m f m2 ->
-     m1 = m2;
+        record_stack_blocks m1 f = Some m2;
 
  extends_same_length_stack:
    forall {injperm: InjectPerm} m1 m2,
@@ -1976,10 +1935,10 @@ record_stack_block_inject_flat {injperm: InjectPerm}:
          forall (o : Z) (k : perm_kind) (p : permission), perm m2 b o k p -> (0 <= o < frame_size fi)%Z)
      (EQINF: forall (b1 b2 : block) (delta : Z), j b1 = Some (b2, delta) -> in_frame f1 b1 <-> in_frame f2 b2)
      (EQsz: frame_adt_size f1 = frame_adt_size f2)
-     (RSB: record_stack_blocks m1 f1 m1')
+     (RSB: record_stack_blocks m1 f1 = Some m1')
      (TNF: top_tframe_no_perm (perm m2) (stack_adt m2)),
      exists m2',
-       record_stack_blocks m2 f2 m2' /\
+       record_stack_blocks m2 f2 = Some m2' /\
        inject j (flat_frameinj (length (Mem.stack_adt m1'))) m1' m2' /\
        (length (Mem.stack_adt m1) = length (Mem.stack_adt m2) ->
         length (Mem.stack_adt m1') = length (Mem.stack_adt m2'));
@@ -2000,7 +1959,7 @@ mem_inject_tailcall_inlined {injperm: InjectPerm}:
       m' (FREE: Mem.free m stk 0 szstk = Some m') 
       (* m'' (USB: Mem.unrecord_stack_block m' = Some m'' ) *)
       m'1 stk0 szstk0 (ALLOC: Mem.alloc m' 0 szstk0 = (m'1, stk0))
-      stkreq m''0 (RSB: Mem.record_stack_blocks m'1 (make_singleton_frame_adt stk0 szstk0 stkreq) m''0)
+      stkreq m''0 (RSB: Mem.record_stack_blocks m'1 (make_singleton_frame_adt stk0 szstk0 stkreq) = Some m''0)
       sp' delta (Fstk: F stk = Some (sp', delta))
       delta0
       (LE: (delta <= delta0)%Z)
@@ -2028,7 +1987,7 @@ mem_inject_tailcall_inlined {injperm: InjectPerm}:
 
 record_stack_blocks_tailcall_original_stack:
   forall m1 f1 m2,
-    record_stack_blocks m1 f1 m2 ->
+    record_stack_blocks m1 f1 = Some m2 ->
     exists f r,
       stack_adt m1 = f::r;
 
@@ -2163,7 +2122,7 @@ Qed.
 
 Lemma record_stack_block_unchanged_on:
   forall m bfi m' (P: block -> Z -> Prop),
-    record_stack_blocks m bfi m' ->
+    record_stack_blocks m bfi = Some m' ->
     strong_unchanged_on P m m'.
 Proof.
   intros; eapply record_stack_blocks_mem_unchanged; eauto.
@@ -2171,7 +2130,7 @@ Qed.
 
 Lemma record_stack_block_perm:
   forall m bfi m',
-    record_stack_blocks m bfi m' ->
+    record_stack_blocks m bfi = Some m' ->
     forall b' o k p,
       perm m' b' o k p ->
       perm m b' o k p.
@@ -2182,7 +2141,7 @@ Qed.
 
 Lemma record_stack_block_perm'
   : forall m m' bofi,
-    record_stack_blocks m bofi m' ->
+    record_stack_blocks m bofi = Some m' ->
     forall (b' : block) (o : Z) (k : perm_kind) (p : permission),
       perm m b' o k p -> perm m' b' o k p.
 Proof.
@@ -2192,7 +2151,7 @@ Qed.
 
 Lemma record_stack_block_valid:
   forall m bf m',
-    record_stack_blocks m bf m' ->
+    record_stack_blocks m bf = Some m' ->
     forall b', valid_block m b' -> valid_block m' b'.
 Proof.
   unfold valid_block; intros.
@@ -2202,7 +2161,7 @@ Qed.
 
 Lemma record_stack_block_nextblock:
   forall m bf m',
-    record_stack_blocks m bf m' ->
+    record_stack_blocks m bf = Some m' ->
     nextblock m' = nextblock m.
 Proof.
   intros.
@@ -2212,7 +2171,7 @@ Qed.
 
 Lemma record_stack_block_is_stack_top:
   forall m b fi m',
-    record_stack_blocks m fi m' ->
+    record_stack_blocks m fi = Some m' ->
     in_frame fi b ->
     is_stack_top (stack_adt m') b.
 Proof.
@@ -2501,40 +2460,6 @@ Lemma storev_perm_inv:
 Proof.
   intros; destruct addr; simpl in *; try congruence.
   eapply perm_store_2; eauto.
-Qed.
-
-Lemma do_stores_nextblock :
-  forall l m m',
-    do_stores m l = Some m' ->
-    nextblock m' = nextblock m.
-Proof.
-  induction l; simpl; intros.
-  congruence. repeat destr_in H.
-  eapply storev_nextblock in Heqo. rewrite <- Heqo; eauto.
-Qed.
-
-Lemma do_stores_stack_adt :
-  forall l m m',
-    do_stores m l = Some m' ->
-    stack_adt m' = stack_adt m.
-Proof.
-  induction l; simpl; intros.
-  congruence. repeat destr_in H.
-  eapply IHl in H1; eauto.
-  rewrite H1. eapply storev_stack_adt; eauto.
-Qed.
-
-Lemma do_stores_perm_inv:
-  forall l m m',
-    do_stores m l = Some m' ->
-    forall b o k p,
-      perm m' b o k p ->
-      perm m b o k p.
-Proof.
-  induction l; simpl; intros.
-  congruence. repeat destr_in H.
-  eapply IHl in H0. 2: eauto.
-  eapply storev_perm_inv; eauto.
 Qed.
 
 (* Lemma frameinj_surjective_free_list_unrecord: *)
